\begin{proposition}{Multiplicative Inverse is the Additive
Inverse}{multiplicative_inverse_is_the_additive_inverse}
\[
\left( - 1 \right) \left( - 1 \right) =  1
\]
\end{proposition}
\begin{proof}
    Recall that 
    \begin{gather*}
        1 +  -1 = 0 \\
        \Updownarrow \enspace \text{multiplying by non-zero constant} \\
        \left( -1 \right) \left( 1 + - 1 \right) = \left( - 1 \right) 0 \\
        \Updownarrow  \enspace \text{distributivity}  \\
        \left( - 1 \right) 1 +  \left( - 1 \right) \left( - 1 \right) = 0 \\
        \Updownarrow   \\
        -  1 +  \left( - 1 \right) \left( - 1 \right) = 0 \\
        \Updownarrow \enspace \text{adding same number both sides}    \\
        1 +  \left( - 1 +  \left( - 1 \right) \left( - 1 \right)  \right) = 1 +
        0 \\
        \Updownarrow \enspace \text{associativity} \\
        \left( 1 +  - 1 \right) +  \left( - 1 \right) \left( - 1 \right) =  1 \\
        \Updownarrow \enspace \text{since} \enspace  1 +  - 1 = 0\\
        \left( - 1 \right) \left( - 1 \right) = 1
    \end{gather*}
\end{proof}
