\begin{proposition}{Inverse Image of the Projection
Mapping}{inverse_image_of_the_projection_mapping}
Suppose \( U \subseteq X _{ \beta  }  \)  and \( \pi  _{ \beta  }  : \prod _{
\alpha \in \mathcal{ J }   } X _{ \alpha  }  \to X _{ \beta  }   \) then \( \pi  _{ \beta  } ^{-1} \left( U
\right) = \prod _{ \alpha \in \mathcal{ J }   } S _{ \alpha  }  \) where \( S _{
\beta } = U \) and \( S _{ \alpha  } =  X _{ \alpha  }   \) for \( \alpha \neq \beta  \) 
\end{proposition}
\begin{proof}
    \( \pi  _{ \beta  } ^{-1} \left( U \right) = \left\{ \left( x _{ \alpha  }
    \right) _{ \alpha \in  \mathcal{ J }   } : \pi _{ \beta  } \left( \left( x
    _{ \alpha  }  \right) _{ \alpha  \in  \mathcal{ J }   } \in  U \right)
    \right\} \) which is true so long as \( x _{ \beta  } \in  U \) without any
    restriction on \( x _{ \alpha  }  \) where \( \alpha \neq \beta  \) and
    therefore \( \pi _{ \beta  } ^{-1} \left( U \right) = \prod _{ \alpha \in
    \mathcal{ J }   } S _{ \alpha  }  \) where \( S _{ \alpha  } = X _{ \alpha
    }  \) if \( \alpha  \neq \beta  \) and \( S _{ \beta  } = U \) 
\end{proof}
