\begin{proposition}{Double Negation Equivalence}{double_negation_equivalence}
Let $ \phi  $ be a formula, then $ \phi  $ is equivalent to $ \neg \left( \neg \phi  \right)  $ 
\end{proposition}
\begin{proof}
    Let $ \mathfrak{ A }   $ be $\mathcal{L}$-Structure, and let $ s $ be an assignment function, let's consider what it means for $ \mathfrak{ A } \models \neg \left( \neg \phi  \right)   $ 
    \begin{align*}
        \mathfrak{ A } \models \neg \left( \neg \phi  \right)  &\Leftrightarrow  ~\text{it's false that}~  \mathfrak{ A } \models \neg \phi  \\
                                                               &\Leftrightarrow ~\text{it's false that, it's false that}~ \mathfrak{ A } \models \phi  \\
                                                               &\Leftrightarrow ~\text{it's true that}~  \mathfrak{ A } \models \phi \\
                                                               &\Leftrightarrow  \mathfrak{ A } \models \phi  
    \end{align*}
    And we know that if it's false that it's false, then it's true, because something is either true or false. Thus we've shown that $ \mathfrak{ A } \models \neg \left( \neg \phi  \right)   $ if and only if $ \mathfrak{ A } \models \phi   $ .
\end{proof}
