\begin{proposition}{Negation of a Sigma Formula is a Pi Formula}{negation_of_a_sigma_formula_is_a_pi_formula}
    Suppose $ \sigma  $ is a $ \Sigma  $-formula, then $ \neg \sigma  $ is equivalent 
a $ \Pi $-formula 
\end{proposition}
\begin{proof}
We will proceed by induction on the complexity of the formula, in other words, 
we will do structural induction
    \begin{itemize}
        \item Base Case
        \begin{itemize}
            \item Suppose $ \phi  $ is an atomic $ \Sigma  $-formula, that means
            that it is an atomic formula in the sense of a normal formula,
            therefore it's negation is the negation of an atomic formula and is
            therefore a $ \Pi   $-formula
            \item Suppose $ \phi :\equiv \neg \alpha $ where $ \alpha $ is an
            atomic formula then by
            \hyperref[proposition:double_negation_equivalence]{the fact that
            double negation ``cancels''} we see that $ \phi  $ is equivalent to
            $ \alpha $ which is an atomic formula, and therefore $ \alpha  $ is
            a $ \Pi  $-formula
        \end{itemize}
        \item Induction Step
        \begin{itemize} \item Suppose $ \alpha  $ and $ \beta  $ are $ \Sigma
        $-formulas where the claim holds
            \begin{itemize}
                \item $ \phi :\equiv \alpha \lor \beta  $, then $ \neg \phi $ is 
                equivalent to $ \neg \alpha \land \neg \beta  $ and therefore by
                our induction hypothesis we know that $ \neg \alpha  $ and $
                \neg \beta  $ are equivent to some  $ \Pi  $-formulas $ \pi _{
                \alpha  }  ,  \pi _{ \beta }  $ then $ \phi  $ is equivalent to
                $ \pi _{ \alpha  } \land \pi _{ \beta  }  $ which is a $ \Pi
                $-formula by the third clause.  \item $ \phi :\equiv \alpha
                \land \beta  $ then $ \neg \phi $ is equivalent to $ \neg \alpha
                \lor \neg \beta  $ and by the same argument above, we can see
                that this is a $ \Pi  $-formula \item $ \phi :\equiv \left(
                \forall x < t \right) \alpha $, then it's negation is $ \left(
                \exists x  \right) \left( x < t \land \neg \alpha  \right)  $ by
                our induction hypothesis we know that $ \neg \alpha  $ is
                equivalent to some $ \Pi $-formula $ \pi _{ \neg \alpha  }  $ so $
                \left( \exists x  \right) \left( x < t \land  \neg \alpha
                \right)  $is
                equivalent to $ \left( \exists x  \right) \left( x < t \land \pi
                _{ \neg \alpha  }    \right) \equiv \left( \exists x < t  \right) \pi
                _{ \neg \alpha  }     $ and therefore we may say that $ \phi  $ is 
                equivalent to a $ \Pi  $-formula.
                \item Suppose $ \phi :\equiv \left( \forall x \le t \right)  $
                then $ \neg \phi  $ is equivalent to $ \left( \exists x  \right)
                \neg \left( \left( x < t \lor x = t \right) \rightarrow \alpha
                \right) :\equiv \left( \exists x  \right) \neg \left( \neg
                \left( x < t \lor  x=  t\right) \lor \alpha  \right)    $ which
                is equivalent to $ \left( \exists x  \right) \left( \left( x < t
                \lor x =  t\right) \land \neg \alpha  \right) :\equiv \left(
                \exists x \le t  \right) \neg \alpha    $ and since $ \neg
                \alpha  $ is equivalent to some $ \Pi  $-formula, $ \pi  _{ \neg
                \alpha }  $  by our inductive hypothesis, we know that $ \left(
                \exists x \le  t \right) \pi _{ \neg \alpha  }  $ is a $ \Pi
                $-formula.
                \item Suppose $ \phi :\equiv \left( \exists x < t  \right)
                \alpha  $ then the negation is equivalent to $ \left( \forall x
                \right) \neg \left( \neg \left( x < t \right) \lor \neg \alpha
                \right) :\equiv \left( \forall x \right) \left( x < t
                \rightarrow \neg \alpha  \right) :\equiv \left( \forall x < t
                \right) \neg \alpha  $, and following similar logic as above
                we can see that $ \left( \forall x < t \right) \neg \alpha  $ is
                a $ \Pi  $-formula
                \item $ \phi :\equiv \left( \exists x \le  t  \right) \alpha  $
                the negation is equivalent to $ \left( \forall x \right) \left(
                \neg \left( \left( x < t \right) \lor \left( x =  t \right) \lor
                \neg \alpha \right) \right) :\equiv \left( \forall x \right)
                \left( \left( x < t \right) \lor \left( x =  t \right) \right)
                \rightarrow \neg \alpha  :\equiv \left( \forall x \le t \right)
                \neg \alpha  $ as needed.
            \end{itemize}
        \end{itemize}
    \end{itemize}
\end{proof}
